Adding boolean simplification using BDDs (not proved).
- Add a file BDD.v that contains an implementation of ROBDDs
- Add a file CP.v that implements (Boolean) constant propagation.
- Modify the compilation to add a second phase of CSE (to get rid of some sharing introduced by the constant propagation).

src/bdd.ml
@@ -1,0 +1,138 @@
+type var = string;;
+
+type ('a,'b) map = ('a * 'b) list
+
+type expr = | False | True | N of int
+
+let pp fmt x = match x with 
+  | True -> Format.fprintf fmt "T"
+  | False -> Format.fprintf fmt "F"
+  | N x -> Format.fprintf fmt "%i" x
+
+
+type node = (expr * var * expr)
+
+type bdd =
+    {
+      t : (int , node) map;
+      h : (node, int) map ;
+      next : int
+    }
+  	
+let empty = {t = []; h = []; next = 0}
+
+let node bdd (l : expr) v (h : expr) = 
+  if l = h then l,bdd
+  else 
+    try 
+      N (List.assoc (l,v,h) bdd.h), bdd 
+    with 
+	Not_found -> 	 
+	  let n = (l,v,h) in 
+	  let u = bdd.next in 
+	  let bdd = {t = (u,n) :: bdd.t; 
+		     h = (n,u) :: bdd.h;
+		     next = u + 1} in 
+	  (N u,bdd)
+;;
+      
+module Op = struct
+    
+  let rec andb bdd (a : expr) (b : expr) : expr * bdd =
+    match a,b with 
+      | False, _ | _, False -> False, bdd
+      | True, f | f, True -> f, bdd
+      | N a, N b -> 
+	let (l1,v1,h1) = List.assoc a bdd.t  in 
+	let (l2,v2,h2) = List.assoc b bdd.t  in 
+	if v1 = v2
+	then 
+	  let (x,bdd) = andb bdd l1 l2 in 
+	  let (y,bdd) = andb bdd h1 h2 in 
+	  node bdd x v1 y
+	else if v1 < v2 then 
+	  let x,bdd = andb bdd l1 (N b) in 
+	  let y,bdd = andb bdd h1 (N b) in 
+	  node bdd x v1 y
+	else 	
+	  let x,bdd = andb bdd (N a) l2 in 
+	  let y,bdd = andb bdd (N a) h2 in 
+	  node bdd x v2 y
+
+  let rec orb bdd (a : expr) (b : expr) : expr * bdd =
+    match a,b with 
+      | False, f | f, False -> f, bdd
+      | True, _ | _, True -> True, bdd
+      | N a, N b -> 
+	let (l1,v1,h1) = List.assoc a bdd.t  in 
+	let (l2,v2,h2) = List.assoc b bdd.t  in 
+	if v1 = v2
+	then 
+	  let (x,bdd) = orb bdd l1 l2 in 
+	  let (y,bdd) = orb bdd h1 h2 in 
+	  node bdd x v1 y
+	else if v1 < v2 then 
+	  let x,bdd = orb bdd l1 (N b) in 
+	  let y,bdd = orb bdd h1 (N b) in 
+	  node bdd x v1 y
+	else 	
+	  let x,bdd = orb bdd (N a) l2 in 
+	  let y,bdd = orb bdd (N a) h2 in 
+	  node bdd x v2 y
+
+
+  let rec negb bdd a  =
+    match a with 
+      | True -> False,bdd
+      | False -> True,bdd
+      | N a -> 	
+	let (l,v,h) = List.assoc a bdd.t  in 
+	let x, bdd = negb bdd l in 
+	let y, bdd = negb bdd h in 
+	node bdd x v y
+
+  let var bdd a =
+    node bdd False a True
+
+  type t = bdd -> expr * bdd
+
+  let (&&) (a : t) (b : t) : t = fun bdd -> 
+    let (a, bdd) = a bdd in 
+    let (b, bdd) = b bdd in 
+    andb bdd a b
+
+  let (||) (a : t) (b : t) : t = fun bdd -> 
+    let (a, bdd) = a bdd in 
+    let (b, bdd) = b bdd in 
+    orb bdd a b
+    
+  let not (a : t) : t = fun bdd -> 
+    let (a,bdd) = a bdd in negb bdd a
+			
+  let run (a : t) x : expr * bdd = a x 
+
+  let var x : t = fun bdd -> var bdd x
+    
+  let (=>) a b = not a || b
+    
+end      
+ 
+
+
+let middle x = Op.(x || not x) 
+let contradiction x = Op.(not (x && not x))
+let chain x y = Op.(x || not y)
+
+  
+  
+let _ = 
+  let test x = Op.(x || (not x )) in 
+  Op.(run (test (var "x" && var "y" || var "x")) empty)
+
+let _ =
+  Op.(run (chain (var "x") (chain (var "y") (chain (var "z") (var "x"))) || not (var "x")) empty)
+
+let _ = Op.(run (var "x" || not (not (var "x"))) empty )
+
+let _ = Op.(run ((var "a" && var "b" && var "c") => var "a") empty);;
+  
