src/BDD.v
@@ -1,0 +1,253 @@
+Require Import Common ZArith. 
+
+Inductive expr := | F | T | N : positive -> expr. 
+
+Notation var := nat. 
+
+Definition node := (expr * var * expr)%type. 
+
+Definition expr_eqb a b :=
+  match a,b with 
+    | T,T => true
+    | F,F => true
+    | N x, N y => (x =? y)%positive
+    | _, _ => false
+  end. 
+
+Definition node_eqb (a b: node) :=
+  match a with 
+    | (xa,ya,za) => 
+        match b with 
+          | (xb,yb,zb) => (expr_eqb xa xb && (NPeano.Nat.eqb ya yb) && expr_eqb za zb)%bool
+        end
+  end. 
+
+Fixpoint assoc {A B} (eq: A -> A ->  bool) x l : option B :=
+  match l with 
+    | nil => None
+    | cons (u,v) q => if eq x u then Some v else assoc eq x q
+  end. 
+
+Module Inner. 
+
+  Record BDD :=
+    {
+      tmap : list (positive * node)%type;
+      hmap : list (node * positive)%type;
+      next : positive
+    }. 
+
+  Definition empty :=
+    {|
+      tmap := nil;
+      hmap := nil;
+      next := 1
+    |}.
+         
+
+  Definition mk_node bdd (l : expr) v (h : expr) :=
+    if expr_eqb l  h then (l,bdd)
+    else
+      match assoc node_eqb (l,v,h) (hmap bdd) with 
+          | Some x => (N x, bdd)
+          | None => let n := (l,v,h) in 
+                    let u := next bdd in 
+                    let bdd := {|  tmap := (u,n) :: tmap bdd;
+                                    hmap := (n,u) :: hmap bdd;
+                                    next := (u + 1)%positive |} in
+                      (N u, bdd)
+       end. 
+
+  Fixpoint andb bdd depth (a b : expr) : option (expr * BDD) :=
+    match depth with 
+      | 0 => None
+      | S depth => 
+          match a,b with 
+            | F, _ => Some (F, bdd)
+            | _, F => Some (F, bdd)
+            | T, x => Some (x, bdd)
+            | x, T => Some (x, bdd)
+            | N na, N nb => 
+                do na <- assoc Pos.eqb na (tmap bdd);
+                do nb <- assoc Pos.eqb nb (tmap bdd);
+                match na,nb with 
+                  | (l1,v1,h1),(l2,v2,h2) =>
+                      match NPeano.Nat.compare v1  v2 with 
+                          | Eq =>
+                              do (x,bdd) <- andb bdd depth l1 l2;
+                              do (y,bdd) <- andb bdd depth h1 h2;
+                              Some (mk_node bdd x v1 y)
+                          | Lt =>
+                              do (x,bdd) <- andb bdd depth l1 b;
+                              do (y,bdd) <- andb bdd depth h1 b;
+                              Some (mk_node bdd x v1 y)
+                          | _ => 
+                              do (x,bdd) <- andb bdd depth a l2;
+                              do (y,bdd) <- andb bdd depth a h2;
+                              Some (mk_node bdd x v2 y)
+                end
+          end
+    end
+       end.
+
+  Fixpoint orb bdd depth (a b : expr) : option (expr * BDD) :=
+    match depth with 
+      | 0 => None
+      | S depth => 
+          match a,b with 
+            | F, x => Some (x, bdd)
+            | x, F => Some (x, bdd)
+            | T, _ => Some (T, bdd)
+            | _, T => Some (T, bdd)
+            | N na, N nb => 
+                do na <- assoc Pos.eqb na (tmap bdd);
+                do nb <- assoc Pos.eqb nb (tmap bdd);
+                match na,nb with 
+                  | (l1,v1,h1),(l2,v2,h2) =>
+                      match NPeano.Nat.compare v1  v2 with 
+                          | Eq =>
+                              do (x,bdd) <- orb bdd depth l1 l2;
+                              do (y,bdd) <- orb bdd depth h1 h2;
+                              Some (mk_node bdd x v1 y)
+                          | Lt =>
+                              do (x,bdd) <- orb bdd depth l1 b;
+                              do (y,bdd) <- orb bdd depth h1 b;
+                              Some (mk_node bdd x v1 y)
+                          | _ => 
+                              do (x,bdd) <- orb bdd depth a l2;
+                              do (y,bdd) <- orb bdd depth a h2;
+                              Some (mk_node bdd x v2 y)
+                end
+          end
+    end
+       end.
+
+
+
+  Fixpoint negb bdd depth (a : expr) : option (expr * BDD) :=
+    match depth with 
+      | 0 => None
+      | S depth => 
+          match a with 
+            | F => Some (T, bdd)
+            | T => Some (F, bdd)
+            | N na => 
+                do na <- assoc Pos.eqb na (tmap bdd);
+                match na with 
+                  | (l,v,h) =>
+                              do (x,bdd) <- negb bdd depth l;
+                              do (y,bdd) <- negb bdd depth h;
+                              Some (mk_node bdd x v y)
+                end
+          end
+    end.
+
+  Fixpoint xorb bdd depth (a b : expr) : option (expr * BDD) :=
+    match depth with 
+      | 0 => None
+      | S depth => 
+          match a,b with 
+            | F, x => Some (x, bdd)
+            | x, F => Some (x, bdd)
+            | T, x => negb bdd depth x (* is this depth enough ?? *)
+            | x, T => negb bdd depth x (* is this depth enough ?? *)
+            | N na, N nb => 
+                do na <- assoc Pos.eqb na (tmap bdd);
+                do nb <- assoc Pos.eqb nb (tmap bdd);
+                match na,nb with 
+                  | (l1,v1,h1),(l2,v2,h2) =>
+                      match NPeano.Nat.compare v1  v2 with 
+                          | Eq =>
+                              do (x,bdd) <- xorb bdd depth l1 l2;
+                              do (y,bdd) <- xorb bdd depth h1 h2;
+                              Some (mk_node bdd x v1 y)
+                          | Lt =>
+                              do (x,bdd) <- xorb bdd depth l1 b;
+                              do (y,bdd) <- xorb bdd depth h1 b;
+                              Some (mk_node bdd x v1 y)
+                          | _ => 
+                              do (x,bdd) <- xorb bdd depth a l2;
+                              do (y,bdd) <- xorb bdd depth a h2;
+                              Some (mk_node bdd x v2 y)
+                end
+          end
+    end
+       end.
+
+  Definition var bdd x :=
+    mk_node bdd F x T. 
+
+  Fixpoint eval bdd depth env (a: expr) : option bool :=
+    match depth with 
+      | 0 => None
+      | S depth => match a with 
+                      | T => Some true
+                      | F => Some false
+                      | N n => do x <- assoc Pos.eqb n (tmap bdd);
+                          match x with 
+                            | (l,v,h) => 
+                                do b <- List.nth_error env v;
+                                if (b: bool) then eval bdd depth env h
+                                else eval bdd depth env l
+                          end
+                  end
+    end. 
+          
+End Inner.
+
+Record BDD := 
+  mk
+    {
+      content: Inner.BDD;
+      depth: nat
+    }.
+
+Section t.   
+
+
+Definition eval bdd env (a: expr) : option bool :=
+  Inner.eval (content bdd) (depth bdd) env a. 
+
+Definition andb bdd a b :=
+  do (e,r) <- Inner.andb (content bdd) (depth bdd) a b;
+  Some (e,mk r (depth bdd)).
+
+Definition orb bdd a b :=
+  do (e,r) <- Inner.orb (content bdd) (depth bdd) a b;
+  Some (e,mk r (depth bdd)).
+
+Definition negb bdd a  :=
+  do (e,r) <- Inner.negb (content bdd) (depth bdd) a;
+  Some (e, mk r (depth bdd)). 
+
+Definition xorb bdd a b :=
+  do (e,r) <- Inner.xorb (content bdd) (depth bdd) a b;
+  Some (e,mk r (depth bdd)).
+
+Definition ite bdd c l r:=
+  do (cl,bdd)  <- andb bdd c l;
+  do (nc,bdd)  <- negb bdd c;
+  do (ncr,bdd) <- andb bdd nc r;
+  orb bdd cl ncr.
+
+Definition empty := mk Inner.empty 0.
+
+Definition mk_var bdd x :=
+  let (e, r) := Inner.var (content bdd) x in 
+    (e, mk r (S (max x (depth bdd)))). 
+
+End t. 
+
+Definition test :=
+  let bdd := empty in 
+  let (a,bdd) := mk_var bdd 10 in 
+  let (b,bdd) := mk_var bdd 11 in 
+  do (a,bdd) <- orb bdd a b;
+  do (na,bdd) <- negb bdd a;
+  do (r,bdd) <- orb bdd a na;
+  do (nr,bdd) <- negb bdd r;
+  do (nnr,bdd) <- negb bdd nr;
+  do (x, bdd) <- orb bdd nnr a;
+  Some (r, bdd). 
+
+Eval compute in test. 
