src/CP.v
@@ -1,0 +1,225 @@
+Require Import Common Core ZArith. 
+Require BDD.
+(* In this compilation pass, we implement boolean simplification using BDDs. *)
+
+Section t. 
+
+  Variable Phi : state.   
+  Variable Var : type -> Type.
+
+  Inductive toption A : type -> Type :=
+  | SNone : forall t, toption A t
+  | SSome : forall (b: A), toption A Core.Tbool. 
+
+  Arguments SNone {A} t. 
+  Arguments SSome {A} b. 
+
+  Definition bind {A B t} (F: A -> toption B Tbool) (o: toption A t) : toption B t :=
+    match o with
+        | SNone t => SNone t
+        | SSome x => (F x) end. 
+
+  Notation "'dob' X <- A ; B" := 
+  (bind (fun X => B) A)
+    (at level 200, X ident, A at level 100, B at level 200). 
+
+  (* Maybe we have a pointer *)
+  Definition sval := toption BDD.expr. 
+
+  Notation V := (fun t => Var t * sval t)%type.   
+  
+  Inductive bexpr :=
+  | Lift : BDD.expr  -> bexpr
+  | Ite : forall (c l r : BDD.expr), bexpr
+  | And : forall (a b : BDD.expr), bexpr
+  | Or : forall (a b : BDD.expr), bexpr
+  | Xor : forall (a b : BDD.expr), bexpr
+  | Not : forall (a : BDD.expr), bexpr.
+  
+  (* Maybe we have a boolean expression *)
+  Definition bexpro := toption bexpr.   
+  
+  (* bang := lift Lift *)
+  Notation bang := (bind (fun x => SSome (Lift x))). 
+  Notation "!!" := (SNone _). 
+
+  Notation bop op dl:= 
+  (let a := DList.hd dl in 
+   let b := DList.hd (DList.tl dl) in 
+     dob a <- (snd a);
+     dob b <- (snd b);
+     SSome (op a b)). 
+
+  Require Import RTL. 
+  Definition cp_expr t (e : expr Phi V t) : (expr Phi Var t) * (toption bexpr t). 
+  refine (match e with
+            | Evar t x => 
+                match t as ty return V ty -> (expr Phi Var ty) * (toption bexpr ty) with 
+                  | Tbool => fun y => (Evar (fst y), bang (snd y)) 
+                  | t => fun y  => (Evar (fst y), !!) end x
+            | Eread t v => (Eread v, !!)
+            | Eread_rf n t v adr => (Eread_rf v (fst adr), !!)
+            | Ebuiltin tys res f args  => 
+                (Ebuiltin f (DList.map (fun _ x => fst x) args), _)           
+            | Econstant t x => 
+                match t as ty return constant ty -> (expr Phi Var ty * toption bexpr ty) with
+                  | Tbool => fun c => if ( c : bool)
+                                    then (Econstant c, SSome (Lift BDD.T))
+                                    else (Econstant c, SSome (Lift BDD.F))
+                  | t => fun c => (Econstant c, !!) end x
+            | Emux ty c l r => 
+                (_ ,
+                 match ty as t return V t -> V t  -> toption bexpr t with 
+                   | Tbool => fun l r =>  
+                               (dob c <- (snd c);
+                                dob l <- (snd l);
+                                dob r <- (snd r);
+                                SSome (Ite c l r))
+                   | _ => fun _ _ => !! end l r)
+            | Efst l t v => (Efst (fst v) , !!)
+            | Esnd l t v => (Esnd (fst v) , !!)
+            | Enth l t m v => (Enth m (fst v), !!)
+            | Etuple l dl => (Etuple (DList.map (fun _ x => fst x) dl), !!)
+          end). 
+  refine (match f in builtin tys res return DList.T V tys -> toption bexpr res with
+            | BI_andb => fun dl =>  bop And dl
+            | BI_orb  => fun dl =>  bop Or  dl
+            | BI_xorb => fun dl =>  bop Xor dl
+            | BI_negb => fun dl =>  dob e <- (snd (DList.hd dl)); SSome (Not e)
+            | _ => fun _ => !!
+          end args); simpl.
+  refine (match snd c with 
+                   | SSome BDD.T => (Evar (fst l))
+                   | SSome BDD.F => (Evar (fst r))
+                   |  _ => Emux (fst c) (fst l) (fst r) end).  Show Proof.
+  Defined. 
+
+     
+  Record Env := mk
+    {
+      Ebdd : BDD.BDD;
+      Eknown: list (BDD.expr * Var Tbool);
+      Enext: nat
+    }. 
+
+  Definition empty : Env := mk BDD.empty [] 100. 
+  
+  Definition add_bdd (Gamma: Env) (b:bexpr ): option (BDD.expr * Env) :=  
+    match b with
+      | Lift x => Some (x, Gamma)
+      | Ite c l r => 
+          do (r,bdd) <- BDD.ite (Ebdd Gamma) c l r;
+          Some (r, mk bdd (Eknown Gamma) (Enext Gamma))
+      | And a b => 
+          do (r,bdd) <- BDD.andb (Ebdd Gamma) a b;
+          Some (r, mk bdd (Eknown Gamma) (Enext Gamma))
+      | Or a b => 
+          do (r,bdd) <- BDD.orb (Ebdd Gamma) a b;
+          Some (r, mk bdd (Eknown Gamma) (Enext Gamma))
+      | Xor a b => 
+          do (r,bdd) <- BDD.xorb (Ebdd Gamma) a b;
+          Some (r, mk bdd (Eknown Gamma) (Enext Gamma))
+      | Not a => 
+          do (r,bdd) <- BDD.negb (Ebdd Gamma) a;
+          Some (r, mk bdd (Eknown Gamma) (Enext Gamma))
+    end. 
+
+  Definition lookup (Gamma: Env) (b: BDD.expr) : option (Var Tbool) :=
+    BDD.assoc BDD.expr_eqb b (Eknown Gamma). 
+
+  Definition add_env (Gamma: Env) (v:Var Tbool) (b:BDD.expr): Env :=
+    mk (Ebdd Gamma) ((b,v) :: Eknown Gamma) (Enext Gamma). 
+  
+  Definition incr Gamma :=
+    let n := (Enext Gamma) in 
+    let (r, bdd) := BDD.mk_var (Ebdd Gamma) n in
+      (r, mk bdd (Eknown Gamma) (S n)). 
+
+  (* Unfortunately, multiple reads from the same state elements cannot be shared *)
+  Definition cp_telescope {A} (E: Env) (T : telescope Phi V A) : telescope Phi Var A. 
+  refine (let fix cp Gamma T :=
+              match T with
+                | & x => & x
+                | telescope_bind arg b cont => 
+                    let (e,svo) := cp_expr arg b in 
+                      match svo in toption _ arg return 
+                         (Var arg * sval arg -> telescope Phi V A) -> 
+                         expr Phi Var arg -> telescope Phi Var A 
+                      with 
+                        | @SNone  arg => 
+                            match arg as ty return 
+                               (Var ty * sval ty -> telescope Phi V A) -> 
+                               expr Phi Var ty -> telescope Phi Var A 
+                            with 
+                              | Tbool => fun cont e => 
+                                         (
+                                           k :- e; 
+                                           let (ptr, Gamma) := incr Gamma in 
+                                             let Gamma := add_env Gamma k ptr in
+                                             cp Gamma (cont (k, SSome ptr)))
+                              | _ => fun cont e => 
+                                      k :- e; cp Gamma (cont (k, SNone _))
+                            end
+                        | SSome sv => 
+                            (* We have a symbolic value *)
+                            fun cont e =>  
+                              match add_bdd Gamma sv with 
+                                | Some (ptr, Gamma) =>
+                                    (* the symbolic value correspond to a pointer in the bdd *)
+                                    match lookup Gamma ptr with
+                                      | None =>
+                                          (* this pointer does not
+                                          correspond to a value. We
+                                          bind this value, and add it
+                                          to the environment*)
+                                          k :- e;
+                                          let Gamma := add_env Gamma k ptr in 
+                                            cp Gamma (cont (k, SSome ptr))
+                                      | Some old => 
+                                          (* the pointer was already
+                                          associated. No need to bind
+                                          a new value *)
+                                          cp Gamma (cont (old, (SSome ptr))) 
+                                    end
+                                | None => 
+                                    (* adding to the bdd failed. This
+                                    should not happen, but is safe *)
+                                    k :- e; cp Gamma (cont (k,SNone _))
+                              end
+                      end cont e
+              end in cp E T). 
+  Defined. 
+
+
+  Definition cp_effects (eff: effects Phi V) : effects Phi Var :=
+    DList.map
+         (fun (a : sync) (x : (option ∘ effect V) a) =>
+            match x with
+              | Some x0 =>
+                  match x0 in (effect _ s) return ((option ∘ effect Var) s) with
+                    | effect_reg_write t x1 x2 =>
+                        Some (effect_reg_write Var t (fst x1) (fst x2))
+                    | effect_regfile_write n t x1 x2 x3 =>
+                        Some (effect_regfile_write Var n t (fst x1) (fst x2) (fst x3))
+                  end
+              | None => None
+            end) eff. 
+  
+  
+  Definition cp_block  t (b : block Phi V t) : block Phi Var t :=    
+    let b := ( _ :- @Econstant  _ _ Tbool true ;
+               _ :- @Econstant  _ _ Tbool false ;
+               b) in 
+    k :-- cp_telescope empty b;
+    match k with (v,g,e) =>
+                   & (fst v, fst g, cp_effects  e)
+    end. 
+End t. 
+
+Definition Compile Phi t (b : Block Phi t) : Block Phi t :=  
+  fun V => cp_block Phi V t (b _). 
+
+Theorem Compile_correct Phi t b (Hwf : WF Phi t b): forall st Delta,
+  Eval Phi st t (Compile Phi t b) Delta =  Eval Phi st t b Delta. 
+Proof. 
+Admitted. 
