src/Compiler.v
@@ -1,4 +1,4 @@
-Require Core Front IR RTL CSE FirstOrder. 
+Require Core Front IR RTL CSE CP FirstOrder. 
 
 
 Definition Compile Phi t  (a : forall Var, Front.action Phi Var t) : RTL.Block Phi t :=
@@ -26,4 +26,13 @@ Print Assumptions Compile_correct.
 
 Definition Fo_compile Phi t (A : Front.Action Phi t) :  FirstOrder.block Phi t :=
   let x := Compile Phi t A in 
+    FirstOrder.compile Phi t (x _ ).  
+
+
+Definition Fo_CP_compile Phi t (A : Front.Action Phi t) :  FirstOrder.block Phi t :=
+  let x := Compile Phi t A in 
+  let x := CP.Compile Phi t x in 
+    (* Constant propagation may have introduced some extra sharing,
+    and we may have to remove some occurences of Evar *)
+  let x := CSE.Compile Phi t x in 
     FirstOrder.compile Phi t (x _ ).  
